remove kallocfun and clean

kalloc/kalloc.c
@@ -55,10 +55,9 @@ void *kalloc(void)
 
 /// clients
 
-
 #define PGSIZE 4096 // bytes per page - original saved in risc.h
 #define PIPESIZE 512
-typedef unsigned int   uint;
+typedef unsigned int uint;
 
 struct pipe {
   char data[PIPESIZE];
@@ -94,7 +93,6 @@ int kalloc_write_42(void) {
 
 
 int kalloc_write_42_kfree(void) {
-
   int *pa;
   pa = 0;
   pa = (int*)kalloc();           // cast to int pointer
@@ -140,8 +138,6 @@ void *kfree_kfree_kalloc(void *pa1, void *pa2) { // original 3
   return kalloc();
 }
 
-// working in progress
-
 int kalloc_write_42_kfree_kfree(void) {
 
   int *pa;
@@ -156,8 +152,6 @@ int kalloc_write_42_kfree_kfree(void) {
   kfree(pa); // make sure it is free and we are back to scratch
   return 0;
 }
-
-
 
 void *kfree_kfree_kalloc_loop(void *pa_start) { // original 6
   int i = 0;
@@ -185,53 +179,21 @@ void* kfree_loop_kalloc(void *pa_start, int n) { // original 7
 
 
 
+
+
 // working in progress
 
-// not added to client 1 yet -- it is in simple-kfree
-void freerange_while_loop(void *pa_start, void *pa_end) {  // admit on pointer
-  while ((char*)pa_start + PGSIZE <= (char*)pa_end) { 
-      kfree(pa_start);
-      pa_start = (char*)pa_start + PGSIZE;
-  }
-}
-
-// should return pa1
-void *client5(void *pa1, void *pa2) { // original 2
-  kfree(pa1);
-  kfree(pa2);
-  kalloc();
-  return kalloc();
-}
-
-
-
-
-void *client10(void *pa_start, int n) { // original 7
-  int i = 0;
-  while (i < n) {
-      kfree(pa_start);
-      pa_start = (char*)pa_start + PGSIZE;
+int* kalloc_int_array(int n) {
+  int *pa;
+  pa = 0;
+  pa = (int*)kalloc();           // cast to int pointer
+  if (pa) {
+    int i = 0;
+    while (i < n) {
+      pa[i] = 42;
       i++;
+    }
+    return pa; // Return the array to the allocated array
   }
-  return kalloc();
+  return 0;
 }
-
-
-
-// this is basicly doing the same as client original 7
-
-
-// this is allowed..
-void client13(void *pa_start) {
-  kfree(pa_start);
-  kfree(pa_start);
-}
-
-
-// working in progress.. simple version of pipealloc without allocating the files..
-
-
-
-
-
-
