kalloc/Verif_clients.v
@@ -10,23 +10,16 @@ Require Import VC.tactics.
 Require Import VC.kalloc.
 
 
-#[export] Instance CompSpecs : compspecs. make_compspecs kalloc.prog. Defined. (* this is my problem.. *)
 
 Local Open Scope logic.
 
-Definition KF_ASI: funspecs := Kalloc_ASI KF_APD _kalloc _kfree.
-Definition KF_imported_specs:funspecs := nil.
-Definition KF_internal_specs: funspecs := KF_ASI.
-Definition KF_globals gv  sh ls xx original_freelist_pointer: mpred:= ASI_kalloc.mem_mgr KF_APD gv sh ls xx original_freelist_pointer.
-Definition KFVprog : varspecs. mk_varspecs kalloc.prog. Defined.
-Definition KFGprog: funspecs := KF_imported_specs ++ KF_internal_specs.
 
 Definition kalloc_write_pipe_spec : ident * funspec :=
  DECLARE _kalloc_write_pipe
  WITH sh : share, original_freelist_pointer:val, xx:Z, ls:list val, gv:globals
  PRE [ ] 
     PROP () PARAMS() GLOBALS(gv) SEP (KF_globals gv sh ls xx original_freelist_pointer)
- POST [ tvoid ] 
+ POST [ tvoid ]
     PROP ( ) RETURN () SEP (
         (if eq_dec original_freelist_pointer nullval then
             KF_globals gv  sh ls xx original_freelist_pointer *emp
@@ -449,6 +442,29 @@ Definition kfree_loop_kalloc_spec :=
                 n_eq_0_case
                 ).
 
+Definition kalloc_int_array_spec : ident * funspec :=
+    DECLARE _kalloc_int_array
+    WITH sh : share, original_freelist_pointer:val, xx:Z, ls:list val, gv:globals
+    PRE [ ] 
+        PROP () PARAMS() GLOBALS(gv) SEP (KF_globals gv sh ls xx original_freelist_pointer)
+    POST [ tint ] 
+        EX r,
+        PROP ( ) RETURN (r) SEP (
+            (if eq_dec original_freelist_pointer nullval then
+                (!! (r = Vint (Int.repr 0)) &&
+                KF_globals gv  sh ls xx original_freelist_pointer * emp)
+            else
+            EX next ls',
+                (!! (next :: ls' = ls /\
+                    r = Vint (Int.repr 42)
+                    ) &&
+                    data_at sh tint (Vint (Int.repr 42)) original_freelist_pointer *
+                    KF_globals gv  sh ls' xx next
+            )
+            )
+        ).
+Compute (sizeof t_struct_pipe).
+
 Definition KFGprog_clients: funspecs := KFGprog ++ [kalloc_write_pipe_spec; kfree_kalloc_spec; kalloc_write_42_spec; kalloc_write_42_kfree_spec; kfree_loop_spec].
 
 Lemma body_kalloc_write_pipe: semax_body KFVprog KFGprog f_kalloc_write_pipe kalloc_write_pipe_spec.
@@ -462,7 +478,7 @@ forward_call (kalloc_spec_sub KF_APD t_struct_pipe) (gv, sh , ls, xx, original_f
         * rewrite H in H0; auto_contradict.
         * forward. entailer.
     + Intros ab. forward_if.
-        rewrite mem_mgr_split. rewrite my_kalloc_token_split. Intros. rewrite kalloc_token_sz_split.
+        rewrite mem_mgr_split. rewrite type_kalloc_token_split. Intros. rewrite kalloc_token_sz_split.
         Intros. 
         rewrite memory_block_data_at_; auto. rewrite data_at__eq. Intros. forward.
         forward. forward. forward. 
@@ -472,6 +488,14 @@ forward_call (kalloc_spec_sub KF_APD t_struct_pipe) (gv, sh , ls, xx, original_f
         rewrite mem_mgr_split. entailer.
         * forward. entailer.
 Qed.
+
+Ltac simplify_kalloc_token :=
+  repeat (
+    rewrite kalloc_token_sz_split;
+    unfold type_kalloc_token
+  );
+  entailer!.
+
 
 Lemma body_kfree_kalloc: semax_body KFVprog KFGprog f_kfree_kalloc kfree_kalloc_spec.
 Proof.
@@ -510,7 +534,7 @@ forward_call (kalloc_spec_sub KF_APD tint) (gv, sh , ls, xx, original_freelist_p
     + Intros ab.
       destruct ls; auto_contradict.
       forward_if.
-        * unfold my_kalloc_token. rewrite kalloc_token_sz_split. Intros.
+        * unfold type_kalloc_token. rewrite kalloc_token_sz_split. Intros.
         rewrite memory_block_data_at_; auto. rewrite data_at__eq. forward.
         forward. forward.
         Exists (Vint(Int.repr 42)) (fst ab) (snd ab). entailer.
@@ -530,12 +554,12 @@ Proof.
     + Intros ab.
       destruct ls; auto_contradict.
       forward_if.
-        * unfold my_kalloc_token. rewrite kalloc_token_sz_split. Intros.
+        * unfold type_kalloc_token. rewrite kalloc_token_sz_split. Intros.
         rewrite memory_block_data_at_; auto. rewrite data_at__eq. Intros. forward.
         forward. 
         forward_call (kfree_spec_sub KF_APD tint) (original_freelist_pointer, gv, sh , snd ab, xx, (fst ab)). (* call kfree *)
         -- if_tac_auto_contradict.
-            unfold my_kalloc_token. rewrite kalloc_token_sz_split. entailer!.
+            unfold type_kalloc_token. rewrite kalloc_token_sz_split. entailer!.
             sep_apply data_at_memory_block. entailer!.
         -- if_tac_auto_contradict.
             forward. Exists (Vint (Int.repr 42)).
@@ -635,9 +659,9 @@ forward_call (kfree_spec_sub KF_APD t_run) (pa1, gv, sh , ls, xx, original_freel
             -- if_tac_auto_contradict. forward_call (kalloc_spec_sub KF_APD t_run) (gv, sh , snd ab, xx, fst ab). (* kalloc *)
                 if_tac.
                     ++ forward. Exists (fst ab) (fst ab) (snd ab). if_tac.
-                        ** unfold KF_globals. unfold my_kalloc_token. entailer!. repeat right. split; auto.
+                        ** unfold KF_globals. unfold type_kalloc_token. entailer!. repeat right. split; auto.
                         ** entailer.
-                    ++ Intros ab0. forward. Exists (fst ab). unfold my_kalloc_token. rewrite mem_mgr_split. 
+                    ++ Intros ab0. forward. Exists (fst ab). unfold type_kalloc_token. rewrite mem_mgr_split. 
                         Exists (fst ab) (snd ab). if_tac_auto_contradict. Exists (fst ab0) (snd ab0). rewrite mem_mgr_split; entailer!.
                         repeat right; split; auto.
 -if_tac_auto_contradict. unfold KF_globals. entailer!.
@@ -645,21 +669,21 @@ forward_call (kfree_spec_sub KF_APD t_run) (pa1, gv, sh , ls, xx, original_freel
 + if_tac_auto_contradict. entailer!.
 + if_tac_auto_contradict. 
     * forward_call (kfree_spec_sub KF_APD t_run) (pa2, gv, sh , ls, xx, original_freelist_pointer). (* call kfree *)
-        -- if_tac_auto_contradict. unfold my_kalloc_token. entailer!.
+        -- if_tac_auto_contradict. unfold type_kalloc_token. entailer!.
         -- if_tac_auto_contradict. forward_call (kalloc_spec_sub KF_APD t_run) (gv, sh , (original_freelist_pointer :: ls), xx, pa2). (* kalloc *)
             if_tac.
                 ++ forward.
                 ++ Intros ab. destruct ls; auto_contradict;
-                    forward; unfold my_kalloc_token, KF_globals; inversion H6; rewrite H3; rewrite H9; Exists pa2; entailer!;
+                    forward; unfold type_kalloc_token, KF_globals; inversion H6; rewrite H3; rewrite H9; Exists pa2; entailer!;
                     do 4 right; left; split; auto.
     * Intros ab. destruct ls; auto_contradict.  
     forward_call (kfree_spec_sub KF_APD t_run) (pa2, gv, sh , snd ab, xx, fst ab). (* call kfree *)
-        -- if_tac_auto_contradict. unfold my_kalloc_token at 2. rewrite kalloc_token_sz_split. entailer!.
+        -- if_tac_auto_contradict. unfold type_kalloc_token at 2. rewrite kalloc_token_sz_split. entailer!.
         -- if_tac_auto_contradict. rewrite mem_mgr_split. Intros. forward_call (kalloc_spec_sub KF_APD t_run) (gv, sh , fst ab::snd ab, xx, pa2). (* kalloc *)
-            ++ unfold my_kalloc_token. rewrite mem_mgr_split.  entailer!.
-            ++ forward. if_tac_auto_contradict. Intros ab0. Exists pa2 (fst ab0) (snd ab0). rewrite mem_mgr_split. unfold KF_globals, my_kalloc_token. rewrite mem_mgr_split. entailer!.
+            ++ unfold type_kalloc_token. rewrite mem_mgr_split.  entailer!.
+            ++ forward. if_tac_auto_contradict. Intros ab0. Exists pa2 (fst ab0) (snd ab0). rewrite mem_mgr_split. unfold KF_globals, type_kalloc_token. rewrite mem_mgr_split. entailer!.
                do 4 right. left; split; auto.
-- if_tac_auto_contradict. unfold KF_globals. rewrite kalloc_token_sz_split. unfold my_kalloc_token. rewrite kalloc_token_sz_split. entailer!.
+- if_tac_auto_contradict. unfold KF_globals. rewrite kalloc_token_sz_split. unfold type_kalloc_token. rewrite kalloc_token_sz_split. entailer!.
 - if_tac_auto_contradict.
     forward_call (kalloc_spec_sub KF_APD t_run) (gv, sh , original_freelist_pointer::ls, xx, pa1). (* kalloc *)
     if_tac_auto_contradict.
@@ -669,21 +693,21 @@ forward_call (kfree_spec_sub KF_APD t_run) (pa1, gv, sh , ls, xx, original_freel
     ++ if_tac_auto_contradict. forward_call (kalloc_spec_sub KF_APD t_run) (gv, sh , snd ab, xx, fst ab). (* kalloc *)
         forward. if_tac_auto_contradict; inversion H5.
         ** Exists (fst ab). if_tac_auto_contradict.
-        unfold my_kalloc_token, KF_globals. entailer!.
+        unfold type_kalloc_token, KF_globals. entailer!.
         do 2 right; left; split; auto.
         ** Intros ab0. Exists (fst ab). if_tac_auto_contradict.
-            Exists (fst ab0) (snd ab0). unfold my_kalloc_token, KF_globals. entailer!.
+            Exists (fst ab0) (snd ab0). unfold type_kalloc_token, KF_globals. entailer!.
             do 3 right; left; split; auto.
-- if_tac_auto_contradict. unfold KF_globals. unfold my_kalloc_token. entailer!.
+- if_tac_auto_contradict. unfold KF_globals. unfold type_kalloc_token. entailer!.
 - if_tac_auto_contradict. forward_call (kalloc_spec_sub KF_APD t_run) (gv, sh , original_freelist_pointer::ls, xx, pa1). (* kalloc *)
     if_tac_auto_contradict.
     Intros ab.
     forward_call (kfree_spec_sub KF_APD t_run) (pa2, gv, sh , snd ab, xx, fst ab). (* call kfree *)
-    + if_tac_auto_contradict. unfold my_kalloc_token at 2; entailer!.
+    + if_tac_auto_contradict. unfold type_kalloc_token at 2; entailer!.
     + if_tac_auto_contradict.
     forward_call (kalloc_spec_sub KF_APD t_run) (gv, sh , fst ab::snd ab, xx, pa2). (* kalloc *)
     if_tac_auto_contradict.
-    Intros ab0. forward. Exists pa2. unfold KF_globals. unfold my_kalloc_token; entailer!.
+    Intros ab0. forward. Exists pa2. unfold KF_globals. unfold type_kalloc_token; entailer!.
     inversion H8. rewrite H14, H15. inversion H5. rewrite H16, H17. entailer!.
 Qed.
 
@@ -702,32 +726,32 @@ forward_call (kfree_spec_sub KF_APD t_run) (pa1, gv, sh , ls, xx, original_freel
         if_tac_auto_contradict. 
         * forward. Exists nullval. unfold KF_globals. entailer!.
         * forward. Exists original_freelist_pointer. Exists (fst ab) (snd ab). entailer!. 
-        unfold my_kalloc_token, KF_globals. entailer!.
+        unfold type_kalloc_token, KF_globals. entailer!.
 -if_tac_auto_contradict. unfold KF_globals. entailer!.
 -if_tac_auto_contradict;
 forward_call (kfree_spec_sub KF_APD t_run) (pa2, gv, sh , ls, xx,original_freelist_pointer). (* call kfree*)
-+ if_tac_auto_contradict. entailer!. unfold my_kalloc_token; entailer!. 
++ if_tac_auto_contradict. entailer!. unfold type_kalloc_token; entailer!. 
 + if_tac_auto_contradict.
     forward_call (kalloc_spec_sub KF_APD t_run) (gv, sh , original_freelist_pointer::ls, xx, pa2). (* kalloc *)
     if_tac_auto_contradict. 
     forward. Exists pa2. unfold KF_globals. entailer!.
         * do 3 right. split; auto.
-        * unfold my_kalloc_token. entailer!. inversion H0. rewrite H9, H10. entailer.
-- if_tac_auto_contradict. unfold KF_globals, my_kalloc_token. entailer!.
+        * unfold type_kalloc_token. entailer!. inversion H0. rewrite H9, H10. entailer.
+- if_tac_auto_contradict. unfold KF_globals, type_kalloc_token. entailer!.
 - if_tac_auto_contradict. 
 forward_call (kfree_spec_sub KF_APD t_run) (pa2, gv, sh , original_freelist_pointer::ls, xx,pa1). (* call kfree*)
 + if_tac_auto_contradict. entailer!.
 + if_tac_auto_contradict. forward_call (kalloc_spec_sub KF_APD t_run) (gv, sh , original_freelist_pointer::ls, xx, pa1). (* kalloc *)
     if_tac_auto_contradict.
-    Intros ab. forward. Exists pa1. unfold my_kalloc_token, KF_globals. entailer!.
+    Intros ab. forward. Exists pa1. unfold type_kalloc_token, KF_globals. entailer!.
     * do 2 right; left; split; auto.
     * inversion H6. rewrite H9, H10. entailer.
-- if_tac_auto_contradict. unfold my_kalloc_token, KF_globals. entailer!.
+- if_tac_auto_contradict. unfold type_kalloc_token, KF_globals. entailer!.
 - if_tac_auto_contradict. forward_call (kfree_spec_sub KF_APD t_run) (pa2, gv, sh , original_freelist_pointer::ls, xx,pa1). (* call kfree*)
-    + if_tac_auto_contradict. unfold my_kalloc_token. entailer!.
+    + if_tac_auto_contradict. unfold type_kalloc_token. entailer!.
     + if_tac_auto_contradict. forward_call (kalloc_spec_sub KF_APD t_run) (gv, sh , pa1::original_freelist_pointer::ls, xx, pa2). (* kalloc *)
     if_tac_auto_contradict. Intros ab.
-    forward. Exists pa2. unfold KF_globals, my_kalloc_token. entailer!.
+    forward. Exists pa2. unfold KF_globals, type_kalloc_token. entailer!.
     inversion H6.
     entailer.
 Qed.
@@ -750,12 +774,12 @@ Proof.
     + Intros ab.
       destruct ls; auto_contradict.
       forward_if.
-        * unfold my_kalloc_token. rewrite kalloc_token_sz_split. Intros.
+        * unfold type_kalloc_token. rewrite kalloc_token_sz_split. Intros.
         rewrite memory_block_data_at_; auto. rewrite data_at__eq. Intros. forward.
         forward. 
         forward_call (kfree_spec_sub KF_APD tint) (original_freelist_pointer, gv, sh , snd ab, xx, (fst ab)). (* call kfree *)
         -- if_tac_auto_contradict.
-            unfold my_kalloc_token. rewrite kalloc_token_sz_split. entailer!.
+            unfold type_kalloc_token. rewrite kalloc_token_sz_split. entailer!.
             sep_apply data_at_memory_block. entailer!.
         -- if_tac_auto_contradict.
             forward. Exists (Vint (Int.repr 42)).
@@ -801,7 +825,7 @@ Proof.
         + forward_call (kfree_spec_sub KF_APD t_run) (p_tmp, gv, sh , (tmp_added_elem ++ ls), xx,curr_head). (* call kfree*)
             * if_tac; destruct H0 as [H01 [H02 [H03 [H04 H05]]]]; rewrite H04 in H1.
                 -- unfold offset_val in H1. destruct pa1; auto_contradict.
-                --unfold KF_globals. unfold my_kalloc_token. rewrite kalloc_token_sz_split. simpl. rewrite kalloc_token_sz_split. Intros.
+                --unfold KF_globals. unfold type_kalloc_token. rewrite kalloc_token_sz_split. simpl. rewrite kalloc_token_sz_split. Intros.
                 entailer!.
             * destruct H0 as [H01 [H02 [H03 [H04 H05]]]]; rewrite H04. unfold is_pointer_or_null.
               unfold offset_val. destruct pa1; auto_contradict; auto.
@@ -853,7 +877,7 @@ Proof.
             apply isptr_offset_val'; auto.
         }
         rewrite H1 in H2; auto_contradict.
-        Intros ab. unfold my_kalloc_token, KF_globals. 
+        Intros ab. unfold type_kalloc_token, KF_globals. 
         inversion H2. entailer!.
 Qed.
 
@@ -896,7 +920,7 @@ Intros. forward. (*forward. unfold abb iate in POSTCONDITION.*)
         (*forward_call (sh, p_tmp, curr_head, xx, gv, (tmp_added_elem ++ ls), PGSIZE). (* call kfree1 *)*)
             *if_tac; destruct H0 as [H001 [H002 [H003 [H04 H05]]]]. rewrite H04 in H.
             -- unfold offset_val in H. destruct pa1; auto_contradict.
-            --unfold KF_globals. unfold my_kalloc_token. rewrite kalloc_token_sz_split. simpl. rewrite kalloc_token_sz_split. Intros.
+            --unfold KF_globals. unfold type_kalloc_token. rewrite kalloc_token_sz_split. simpl. rewrite kalloc_token_sz_split. Intros.
             entailer!.
             * destruct H0 as [H001 [H002 [H003 [H04 H05]]]]. rewrite H04.
                 assert ( isptr (offset_val (i * PGSIZE) pa1)). {apply isptr_offset_val'. auto. }
@@ -990,11 +1014,11 @@ destruct H as [H11 [H12 H13]]; auto.
                     **  simpl in H0. rewrite H0 in H3. inversion H3.
                     ** simpl in H1. simpl in H0. Exists (fst ab) (snd ab). unfold KF_globals. rewrite H1.
                     entailer!. rewrite H0 in H3. rewrite app_nil_l in H3. auto.
-                    unfold my_kalloc_token. entailer!.
+                    unfold type_kalloc_token. entailer!.
             -- Exists (fst vret) (snd vret).
                 entailer.
                 destruct (0 <? n) eqn:etrue; try rep_lia.
-                unfold KF_globals. unfold my_kalloc_token. entailer!.
+                unfold KF_globals. unfold type_kalloc_token. entailer!.
                 destruct (snd vret).
                 ++ replace (S n0) with (n0 + 1)%nat in H0; try rep_lia. 
                 destruct n0 eqn:en0.
