kalloc/Verif_kalloc_kfree.v
@@ -1,23 +1,13 @@
 Require Import VST.floyd.proofauto.
+Require Import VC.tactics.
 Require Import VC.ASI_kalloc.
 Require Import VC.kalloc.
-Require Import VC.kallocfun.
-Require Import VC.tactics.
 Require Import VC.Spec_kalloc.
-
-(*#[export] Instance CompSpecs : compspecs. make_compspecs prog. Defined.
-Definition Vprog : varspecs. mk_varspecs prog. Defined.*)
-
-
-
-(*Require Import malloc.
-Require Import malloc_lemmas.
-Require Import malloc_sep.*)
 Require Import VC.kalloc_kfree_definitions.
 
 Local Open Scope logic.
 
-Lemma body_kfree: semax_body MF_Vprog MF_Gprog f_kfree (kfree_spec KF_APD t_run).
+Lemma body_kfree: semax_body KFVprog KFGprog f_kfree (kfree_spec KF_APD t_run).
 Proof. start_function. Intros.
 forward.
 rewrite mem_mgr_split. Intros.
@@ -26,19 +16,16 @@ destruct (eq_dec new_head nullval).
     * rewrite e in H2; auto_contradict.
     * forward. entailer. rewrite mem_mgr_split. entailer.
 - forward_if.
-    * Intros. forward. unfold my_kalloc_token. Intros. rewrite kalloc_token_sz_split. Intros. 
-    rewrite memory_block_data_at_; auto. forward. forward. 
-    (*forward. intros. rewrite kalloc_token_sz_split. Intros.
-    rewrite memory_block_data_at_.
-     forward.*) entailer. rewrite mem_mgr_split. refold_freelistrep. entailer!.
+    * Intros. forward. unfold type_kalloc_token. Intros. rewrite kalloc_token_sz_split. Intros. 
+     rewrite memory_block_data_at_; auto. forward. forward. 
+     entailer. rewrite mem_mgr_split. refold_freelistrep. entailer!.
      right; split; auto. unfold not; auto_contradict.
     * forward. entailer.
 Qed.
 
-
-Lemma body_kalloc: semax_body MF_Vprog MF_Gprog f_kalloc (kalloc_spec (KF_APD) t_run).
+Lemma body_kalloc: semax_body KFVprog KFGprog f_kalloc (kalloc_spec (KF_APD) t_run).
 Proof. start_function.
-rewrite mem_mgr_split. Intros. forward.  (*unfold abbreviate in POSTCONDITION.*)
+rewrite mem_mgr_split. Intros. forward.
 forward_if (
     PROP  ( )
     LOCAL (
@@ -52,27 +39,22 @@ forward_if (
         (
           EX next ls',
           (!! (next :: ls' = ls) &&
-              my_kalloc_token KF_APD sh (t_run) original_freelist_pointer *
+              type_kalloc_token KF_APD sh (t_run) original_freelist_pointer *
               ASI_kalloc.mem_mgr KF_APD gv sh ls' xx next
           )
         )
-        (*ASI_kalloc.mem_mgr KF_APD gv sh ls xx original_freelist_pointer*
-                   (if eq_dec original_freelist_pointer nullval
-                   then emp
-                   else my_kalloc_token KF_APD sh t_run original_freelist_pointer)*)
     )
 )%assert.
 - destruct H3 as [[H0011 H0012] | [H0021 H0022]].
     + rewrite H0012 in H4; auto_contradict.
     + destruct ls; auto_contradict.
     refold_freelistrep. Intros.
-    forward. (*unfold abbreviate in POSTCONDITION.*) forward.
+    forward. forward.
     entailer.
-    (*destruct (eq_dec original_freelist_pointer nullval) eqn:e1; auto_contradict. entailer.*)
     rewrite mem_mgr_split. Intros. 
     refold_freelistrep. if_tac.
     * rewrite H11 in H0022; auto_contradict.
-    * entailer. Exists v ls. entailer. unfold my_kalloc_token.
+    * entailer. Exists v ls. entailer. unfold type_kalloc_token.
     rewrite kalloc_token_sz_split. rewrite mem_mgr_split. entailer!.
     -- split. unfold malloc_compatible. destruct original_freelist_pointer; auto_contradict. 
         unfold malloc_compatible in H3. destruct H3. split; auto.
